proof/Scratch.thy
@@ -2,6 +2,65 @@ theory Scratch
   imports Main Observation
 begin
 
-lemma "If a 
+text \<open>So, you can't have a typeclass return a type parameter. Let's see if we can define a type with
+no properties, then later, assert some properties *of* that type and use them in a proof. So... some
+`foo` exists. We don't know what it is.\<close>
 
+typedecl foo
+
+text \<open>We can make a container for foo\<close>
+
+datatype box = Box "foo"
+
+text \<open>We can use foo for equality...\<close>
+
+lemma "(x :: foo) \<noteq> (y :: foo) \<longrightarrow> (Box x) \<noteq> (Box y)"
+  apply auto
+  done
+
+lemma "(x :: foo) = (y :: foo) \<longrightarrow> (Box x) = (Box y)"
+  apply auto
+  done
+
+text \<open>We can define a typeclass which returns foos...\<close>
+
+class openable =
+  fixes open1 :: "'a \<Rightarrow> foo"
+
+instantiation box :: openable
+begin
+primrec open1 :: "box \<Rightarrow> foo" where
+"open1 (Box f) = f"
+instance ..
 end
+
+text \<open>Now it'd be nice if we could show something trivial, like... if foo is, say, a nat, then open1
+returns a nat. If we were using type parameters, I'd make a "box nat", but since we're NOT using
+type parameters... I want to write, like, (foo = nat) \<Rightarrow> is_nat (openable x)" but I have no idea how\<close>
+
+text \<open>I think what I want here is maybe... a locale? Let's try that...\<close>
+
+locale partial_order =
+  fixes le :: "'a \<Rightarrow> 'a \<Rightarrow> bool"
+  assumes refl [intro, simp]: "le x x"
+    and anti_sym [intro]: "\<lbrakk>le x y; le y x\<rbrakk> \<Longrightarrow> x = y"
+    and trans [trans]: "\<lbrakk>le x y; le y z\<rbrakk> \<Longrightarrow> le x z"
+
+text \<open>So... what we've done here is assert a le function exists, and it obeys these laws, but we
+haven't actually said what le is. le could operate over cats or cargo ships. It could be < or >. Can
+I define a locale that returns a type parameter?\<close>
+
+locale openable2 =
+  fixes open2 :: "'a \<Rightarrow> 'b"
+
+text \<open>Huh. So... all I've said here is that a binary function exists. What about... making a box for
+a type parameter? That's something we can't do with typeclasses...\<close>
+
+datatype 'a abstract_box = AbstractBox "'a"
+locale boxable =
+  fixes box :: "'a \<Rightarrow> ('b abstract_box)"
+
+text \<open>Okay, so I can define a boxable function which returns something with type parameters. Note
+that our box is over a different type, so we could, I dunno, take strings and constantly return
+AbstractBox 2 or something.\<close>
+
