proof/LocaleTest.thy
@@ -5,9 +5,26 @@ begin
 (* A box for things of some unspecified type 'a *)
 datatype 'a box = Box "'a"
 
-(* A typeclass that can make boxes? *)
+(* A typeclass that can make boxes?
+
 class boxable =
   fixes makebox :: "'o \<Rightarrow> ('a box)"
+*)
 
 (* This complains "multiple variables in type specification, and I can't seem to parameterize
 the typeclass with type variables itself. Shit. *)
+
+locale menagerie =
+  fixes animal_type :: "'at"
+  and favorite :: "'a"
+begin
+
+(* We can't use animal_type at the type level here, so... while you CAN apparently pass types
+to locales when constructing intepretations, those types can't be used in definitions. Which...
+I guess makes sense, cuz the definitions here should typecheck on their *own*. Right? *)
+definition feed :: "'at \<Rightarrow> bool" where
+"feed a \<equiv> (case a of favorite \<Rightarrow> True | x \<Rightarrow> False)"
+end
+
+interpretation pets: menagerie nat 0 .
+
